smtlink/test-all.lisp
@@ -43,138 +43,138 @@
 (include-book "arithmetic/top-with-meta" :dir :system)
 (include-book "./SMT-connect")
 
-;; ;; test0
-;; (defconst *a* 1)
-;; (defun bar0 (x) (* 2 x))
+;; test0
+(defconst *a* 1)
+(defun bar0 (x) (* 2 x))
 
-;; ;; a very simple theorem
-;; (defthm test0
-;;   (implies (and (and (rationalp x)) (and))
-;; 	   (equal (+ x x) (* *a* (bar0 x))))
-;;   :hints
-;;   (("Goal"
-;;     :clause-processor
-;;     (my-clause-processor clause
-;; 			 '( (:expand ((:functions ((bar0 rationalp)))
-;; 				      (:expansion-level 1)))
-;; 			   (:python-file "test0")
-;; 			   (:let ())
-;; 			   (:hypothesize ())
-;; 			   (:use ((:type ())
-;; 				  (:hypo ())
-;; 				  (:main ()))))
-;; 			 ))))
+;; a very simple theorem
+(defthm test0
+  (implies (and (and (rationalp x)) (and))
+	   (equal (+ x x) (* *a* (bar0 x))))
+  :hints
+  (("Goal"
+    :clause-processor
+    (my-clause-processor clause
+			 '( (:expand ((:functions ((bar0 rationalp)))
+				      (:expansion-level 1)))
+			   (:python-file "test0")
+			   (:let ())
+			   (:hypothesize ())
+			   (:use ((:type ())
+				  (:hypo ())
+				  (:main ()))))
+			 ))))
 
-;; ;; test1
-;; (defun foo1 (x y) (* x (+ 1 y)))
+;; test1
+(defun foo1 (x y) (* x (+ 1 y)))
 
-;; ;; very first piece of test case
-;; (defthm test1 (implies (and (and (rationalp x)
-;; 				 (integerp y)
-;; 				 (integerp z))
-;; 			    (and (not (<= x 0))
-;; 				 (equal z (+ 3/2 4))
-;; 				 (or (> x y) (> x (+ y 40/3)))))
-;; 		       (> (foo1 x (foo1 x z)) (foo1 x y)))
-;;   :hints
-;;   (("Goal"
-;;     :clause-processor
-;;     (my-clause-processor clause
-;; 			 '( (:expand ((:functions ((foo1 rationalp)))
-;; 				      (:expansion-level 1)))
-;; 			   (:python-file "test1")
-;; 			   (:let ())
-;; 			   (:hypothesize ())
-;; 			   (:use ((:type ())
-;; 				  (:hypo ())
-;; 				  (:main ()))))))))
+;; very first piece of test case
+(defthm test1 (implies (and (and (rationalp x)
+				 (integerp y)
+				 (integerp z))
+			    (and (not (<= x 0))
+				 (equal z (+ 3/2 4))
+				 (or (> x y) (> x (+ y 40/3)))))
+		       (> (foo1 x (foo1 x z)) (foo1 x y)))
+  :hints
+  (("Goal"
+    :clause-processor
+    (my-clause-processor clause
+			 '( (:expand ((:functions ((foo1 rationalp)))
+				      (:expansion-level 1)))
+			   (:python-file "test1")
+			   (:let ())
+			   (:hypothesize ())
+			   (:use ((:type ())
+				  (:hypo ())
+				  (:main ()))))))))
 
-;; ;; test2
-;; (defun foo2 (x) (+ x 3))
-;; (defun bar2 (y) (* 2 (foo2 y)))
+;; test2
+(defun foo2 (x) (+ x 3))
+(defun bar2 (y) (* 2 (foo2 y)))
 
-;; (defthm test2
-;;   (implies (and (and (rationalp y))
-;; 		(and (> y 1)))
-;; 	   (> (bar2 (foo2 y)) 12))
-;;   :hints
-;;   (("Goal"
-;;     :clause-processor
-;;     (my-clause-processor clause
-;; 			 '( (:expand ((:functions ((foo2 rationalp)
-;; 						   (bar2 rationalp)))
-;; 				      (:expansion-level 1)))
-;; 			    (:python-file "test2")
-;; 			    (:let ())
-;; 			    (:hypothesize ())
-;; 			    (:use ((:type ())
-;; 				   (:hypo ())
-;; 				   (:main ()))))))))
+(defthm test2
+  (implies (and (and (rationalp y))
+		(and (> y 1)))
+	   (> (bar2 (foo2 y)) 12))
+  :hints
+  (("Goal"
+    :clause-processor
+    (my-clause-processor clause
+			 '( (:expand ((:functions ((foo2 rationalp)
+						   (bar2 rationalp)))
+				      (:expansion-level 1)))
+			    (:python-file "test2")
+			    (:let ())
+			    (:hypothesize ())
+			    (:use ((:type ())
+				   (:hypo ())
+				   (:main ()))))))))
 
-;; ;; test3
-;; (defun foo3 (x args) (+ x (nth 0 args) (nth 1 args)))
+;; test3
+(defun foo3 (x args) (+ x (nth 0 args) (nth 1 args)))
 
-;; (defthm test3
-;;   (implies (and (and (rationalp x)
-;; 		     (integerp i)
-;; 		     (integerp j))
-;; 		(and (> x 0)
-;; 		     (> i 0)
-;; 		     (> j 0)))
-;; 	   (> (foo3 x '(i j)) 0))
-;;   :hints
-;;   (("Goal"
-;;     :clause-processor
-;;     (my-clause-processor clause
-;; 			 '( (:expand ((:functions ((foo3 rationalp)))
-;; 				      (:expansion-level 1)))
-;; 			    (:python-file "test3")
-;; 			    (:let ())
-;; 			    (:hypothesize ())
-;; 			    (:use ((:type ())
-;; 				   (:hypo ())
-;; 				   (:main ()))))))))
+(defthm test3
+  (implies (and (and (rationalp x)
+		     (integerp i)
+		     (integerp j))
+		(and (> x 0)
+		     (> i 0)
+		     (> j 0)))
+	   (> (foo3 x '(i j)) 0))
+  :hints
+  (("Goal"
+    :clause-processor
+    (my-clause-processor clause
+			 '( (:expand ((:functions ((foo3 rationalp)))
+				      (:expansion-level 1)))
+			    (:python-file "test3")
+			    (:let ())
+			    (:hypothesize ())
+			    (:use ((:type ())
+				   (:hypo ())
+				   (:main ()))))))))
 
-;; ;; test4
-;; ;; x^2 + y^2 >= 2xy
-;; ;; a(x,y) = x*y
-;; ;; b(x) = 2*x = (a 2 x)
-;; ;; c(x,y) = x+y
-;; ;; d(x) = x^2 = (a x x)
-;; ;; e(x) = -x
-;; ;; f(x,y) = x-y = (c x -y) = (c x (e y))
-;; (defun a4 (x y) (* x y))
-;; (defun b4 (x) (a4 2 x))
-;; (defun c4 (x y) (+ x y))
-;; (defun d4 (x) (a4 x x))
-;; (defun e4 (x) (- x))
-;; (defun f4 (x y) (c4 x (e4 y)))
+;; test4
+;; x^2 + y^2 >= 2xy
+;; a(x,y) = x*y
+;; b(x) = 2*x = (a 2 x)
+;; c(x,y) = x+y
+;; d(x) = x^2 = (a x x)
+;; e(x) = -x
+;; f(x,y) = x-y = (c x -y) = (c x (e y))
+(defun a4 (x y) (* x y))
+(defun b4 (x) (a4 2 x))
+(defun c4 (x y) (+ x y))
+(defun d4 (x) (a4 x x))
+(defun e4 (x) (- x))
+(defun f4 (x y) (c4 x (e4 y)))
 
-;; (defthm test4
-;;     (implies (and (and (rationalp a)
-;; 		       (rationalp b))
-;; 		  (and))
-;; 	     (>= (f4 (d4 (c4 a b))
-;; 		     (a4 (b4 a) b))
-;; 		 (a4 (b4 a) b)))
-;;   :hints
-;;   (("Goal"
-;;     :clause-processor
-;;     (my-clause-processor clause
-;; 			 '( (:expand ((:functions ((a4 rationalp)
-;; 						   (b4 rationalp)
-;; 						   (c4 rationalp)
-;; 						   (d4 rationalp)
-;; 						   (e4 rationalp)
-;; 						   (f4 rationalp))))
-;; 			             ;;(:expansion-level 1)
-;; 			     )
-;; 			    (:python-file "test4")
-;; 			    (:let ())
-;; 			    (:hypothesize ())
-;; 			    (:use ((:type ())
-;; 				   (:hypo ())
-;; 				   (:main ()))))))))
+(defthm test4
+    (implies (and (and (rationalp a)
+		       (rationalp b))
+		  (and))
+	     (>= (f4 (d4 (c4 a b))
+		     (a4 (b4 a) b))
+		 (a4 (b4 a) b)))
+  :hints
+  (("Goal"
+    :clause-processor
+    (my-clause-processor clause
+			 '( (:expand ((:functions ((a4 rationalp)
+						   (b4 rationalp)
+						   (c4 rationalp)
+						   (d4 rationalp)
+						   (e4 rationalp)
+						   (f4 rationalp))))
+			             ;;(:expansion-level 1)
+			     )
+			    (:python-file "test4")
+			    (:let ())
+			    (:hypothesize ())
+			    (:use ((:type ())
+				   (:hypo ())
+				   (:main ()))))))))
 
 ;; test5: with recursive call
 ;; (fac)
@@ -188,120 +188,121 @@
   (("Goal"
     :clause-processor
     (my-clause-processor clause
-			 '( (:expand ((:functions ((fac integerp)))
+			 '( (:expand ((:functions ((fac integerp)
+						   (zp booleanp)))
 				      (:expansion-level 3)))
 			    (:python-file "test5")
 			    (:let ())
 			    (:hypothesize ())
-                         (:use ((:type ())
-                                (:hypo ())
-                                (:main ()))))))))
+			    (:use ((:type ())
+				   (:hypo ())
+				   (:main ()))))))))
 
 
-;; ;; test6: user given hypothesis
-;; ;; a - real
-;; ;; b - real
-;; ;; gamma - real
-;; ;; m - integer
-;; ;; n - integer
-;; ;; 0 < gamma < 1
-;; ;; 0 < m < n
-;; ;; adapted from test4: a^2 + b^2 >= 2ab
+;; test6: user given hypothesis
+;; a - real
+;; b - real
+;; gamma - real
+;; m - integer
+;; n - integer
+;; 0 < gamma < 1
+;; 0 < m < n
+;; adapted from test4: a^2 + b^2 >= 2ab
 
-;; ;; 2*a*b*gamma^n <= -2*a*b*gamma^m + ...???
-;; (defun a6 (x y) (* x y))
-;; (defun b6 (x) (a6 2 x))
-;; (defun c6 (x y) (+ x y))
-;; (defun d6 (x) (a6 x x))
-;; (defun e6 (x) (- x))
-;; (defun f6 (x y) (c6 x (e6 y)))
-;; (defun foo6 (x n) (expt x n))
+;; 2*a*b*gamma^n <= -2*a*b*gamma^m + ...???
+(defun a6 (x y) (* x y))
+(defun b6 (x) (a6 2 x))
+(defun c6 (x y) (+ x y))
+(defun d6 (x) (a6 x x))
+(defun e6 (x) (- x))
+(defun f6 (x y) (c6 x (e6 y)))
+(defun foo6 (x n) (expt x n))
 
-;; (defthm test6
-;;     (implies (and (and (rationalp a)
-;; 		       (rationalp b)
-;; 		       (rationalp gamma)
-;; 		       (integerp m)
-;; 		       (integerp n))
-;; 		  (and (> gamma 0)
-;; 		       (< gamma 1)
-;; 		       (> m 0)
-;; 		       (< m n)))
-;; 	     (>= (a6 (expt gamma m)
-;; 		    (f6 (d6 (c6 a b))
-;; 			(a6 (b6 a) b)))
-;; 		 (a6 (foo6 gamma n)
-;; 		    (a6 (b6 a) b))))
-;;   :hints
-;;   (("Goal"
-;;     :clause-processor
-;;     (my-clause-processor clause
-;; 			 '( (:expand ((:functions ((a6 rationalp)
-;; 						   (b6 rationalp)
-;; 						   (c6 rationalp)
-;; 						   (d6 rationalp)
-;; 						   (e6 rationalp)
-;; 						   (f6 rationalp)
-;; 						   (foo6 rationalp))))
-;; 				      (:expansion-level 1)))
-;; 			    (:python-file "test6")
-;; 			    (:let ((expt_gamma_m (expt gamma m) rationalp)
-;; 				   (expt_gamma_n (expt gamma n) rationalp)))
-;; 			    (:hypothesize ((< expt_gamma_n expt_gamma_m)
-;; 					   (> expt_gamma_m 0)
-;; 					   (> expt_gamma_n 0)))
-;; 			    (:use ((:type ())
-;; 				   (:hypo ())
-;; 				   (:main ()))))))))
+(defthm test6
+    (implies (and (and (rationalp a)
+		       (rationalp b)
+		       (rationalp gamma)
+		       (integerp m)
+		       (integerp n))
+		  (and (> gamma 0)
+		       (< gamma 1)
+		       (> m 0)
+		       (< m n)))
+	     (>= (a6 (expt gamma m)
+		    (f6 (d6 (c6 a b))
+			(a6 (b6 a) b)))
+		 (a6 (foo6 gamma n)
+		    (a6 (b6 a) b))))
+  :hints
+  (("Goal"
+    :clause-processor
+    (my-clause-processor clause
+			 '( (:expand ((:functions ((a6 rationalp)
+						   (b6 rationalp)
+						   (c6 rationalp)
+						   (d6 rationalp)
+						   (e6 rationalp)
+						   (f6 rationalp)
+						   (foo6 rationalp))))
+				      (:expansion-level 1))
+			    (:python-file "test6")
+			    (:let ((expt_gamma_m (expt gamma m) rationalp)
+				   (expt_gamma_n (expt gamma n) rationalp)))
+			    (:hypothesize ((< expt_gamma_n expt_gamma_m)
+					   (> expt_gamma_m 0)
+					   (> expt_gamma_n 0)))
+			    (:use ((:type ())
+				   (:hypo ())
+				   (:main ()))))))))
 
-;; ;; test7: user given hints
-;; ;; Design:
-;; ;; '( (:expand (...))
-;; ;;    (:python-file "..")
-;; ;;    (:let ((...)
-;; ;;           (...)))
-;; ;;    (:hypothesis ((...)
-;; ;;                  (...)))
-;; ;;    (:use (:type ((...) (...) (...)))
-;; ;;          (:hypo ((...) (...) (...)))
-;; ;;          (:main ((...) (...) (...)))))
-;; ;; Explanation:
-;; ;; The three classes of hints are seperately for types,
-;; ;; hypotheses and the main theorem returned.
-;; ;; Type theorems come from the type statements in let
-;; ;; bindings, hypo theorems come from user provided hypotheses,
-;; ;; and the main theorem is the implication from SMT result
-;; ;; to the initial theorem we want to prove.
-;; ;; Note:
-;; ;; Each theorem can have multiple hints.
-;; ;; 
+;; test7: user given hints
+;; Design:
+;; '( (:expand (...))
+;;    (:python-file "..")
+;;    (:let ((...)
+;;           (...)))
+;;    (:hypothesis ((...)
+;;                  (...)))
+;;    (:use (:type ((...) (...) (...)))
+;;          (:hypo ((...) (...) (...)))
+;;          (:main ((...) (...) (...)))))
+;; Explanation:
+;; The three classes of hints are seperately for types,
+;; hypotheses and the main theorem returned.
+;; Type theorems come from the type statements in let
+;; bindings, hypo theorems come from user provided hypotheses,
+;; and the main theorem is the implication from SMT result
+;; to the initial theorem we want to prove.
+;; Note:
+;; Each theorem can have multiple hints.
+;; 
 
-;; (defthm hint-thm-7-1
+(defthm hint-thm-7-1
+  (implies (and (rationalp x)
+		(rationalp y))
+	   (>= (* (+ x y) (+ x y)) 0))
+  :rule-classes :linear)
+
+;; (defthm hint-thm-7-2
 ;;   (implies (and (rationalp x)
 ;; 		(rationalp y))
-;; 	   (>= (* (+ x y) (+ x y)) 0))
-;;   :rule-classes :linear)
+;; 	   (equal (* (+ x y) (+ x y))
+;; 		  (expt (+ x y) 2))))
 
-;; ;; (defthm hint-thm-7-2
-;; ;;   (implies (and (rationalp x)
-;; ;; 		(rationalp y))
-;; ;; 	   (equal (* (+ x y) (+ x y))
-;; ;; 		  (expt (+ x y) 2))))
-
-;; (defthm test7
-;;   (implies (and (and (rationalp x)
-;; 		     (rationalp y))
-;; 		(and))
-;; 	   (>= (expt (+ x y) 2) 0))
-;;   :hints
-;;   (("Goal"
-;;     :clause-processor
-;;     (my-clause-processor clause
-;; 			 '( (:expand ())
-;; 			    (:python-file "test7")
-;; 			    (:let ((expt_plus_x_y_square (expt (+ x y) 2) rationalp)))
-;; 			    (:hypothesize ((>= expt_plus_x_y_square 0)))
-;; 			    (:use ((:type ())
-;; 			    	   (:hypo ((hint-thm-7-1)))
-;; 			    	   (:main (hint-thm-7-1))))
-;; 			   )))))
+(defthm test7
+  (implies (and (and (rationalp x)
+		     (rationalp y))
+		(and))
+	   (>= (expt (+ x y) 2) 0))
+  :hints
+  (("Goal"
+    :clause-processor
+    (my-clause-processor clause
+			 '( (:expand ())
+			    (:python-file "test7")
+			    (:let ((expt_plus_x_y_square (expt (+ x y) 2) rationalp)))
+			    (:hypothesize ((>= expt_plus_x_y_square 0)))
+			    (:use ((:type ())
+			    	   (:hypo ((hint-thm-7-1)))
+			    	   (:main (hint-thm-7-1))))
+			   )))))
