smtlink/SMT-connect.lisp
@@ -1,4 +1,3 @@
-
 (in-package "ACL2")
 
 (defstub acl2-my-prove (term fn-lst fn-level fname let-expr new-hypo let-hints hypo-hints main-hints) (mv t nil nil nil nil))
@@ -44,7 +43,7 @@
 				   (cadr (assoc ':use hint)))))
 	  (main-hints (cadr (assoc ':main
 				   (cadr (assoc ':use hint))))))
-      (prog2$ (cw "fn-lst: ~q0" fn-lst)
+      (prog2$ (cw "fn-lst: ~q0, fn-level: ~q1" fn-lst fn-level)
       (mv-let (res expanded-cl type-related-theorem hypo-theorem fn-type-theorem)
 	      (acl2-my-prove (disjoin cl) fn-lst fn-level fname let-expr new-hypo let-hints hypo-hints main-hints)
 	      (if res
@@ -61,4 +60,3 @@
   my-clause-processor
   nil
   :ttag my-cl-proc)
-
